Logic/Modal/Basic/Axioms.lean
@@ -1,0 +1,152 @@
+import Logic.Modal.Basic.Formula
+
+lemma _root_.Set.subset_triunion₁ (s₁ s₂ s₃ : Set F) : s₁ ⊆ (s₁ ∪ s₂ ∪ s₃) := Set.Subset.trans
+  (Set.subset_union_left _ _) (Set.subset_union_left _ _)
+
+lemma _root_.Set.subset_triunion₂  (s₁ s₂ s₃ : Set F) : s₂ ⊆ (s₁ ∪ s₂ ∪ s₃) := Set.Subset.trans
+  (Set.subset_union_right _ _) (Set.subset_union_left _ _)
+
+lemma _root_.Set.subset_triunion₃ (s₁ s₂ s₃ : Set F) : s₃ ⊆ (s₁ ∪ s₂ ∪ s₃) := Set.subset_union_right _ _
+
+namespace LO.Modal
+
+variable {F : Type u} [ModalLogicSymbol F]
+
+section Axioms
+
+variable (p q : F)
+
+@[simp] abbrev AxiomK := □(p ⟶ q) ⟶ □p ⟶ □q
+def AxiomK.ctx : Set F := { AxiomK p q | (p) (q) }
+notation "𝐊" => AxiomK.ctx
+@[simp] lemma AxiomK.ctx.includes_AxiomK : (AxiomK p q) ∈ 𝐊 := by simp [ctx]; aesop;
+
+@[simp] abbrev AxiomT := □p ⟶ p
+def AxiomT.ctx : Set F := { AxiomT p | p }
+notation "𝐓" => AxiomT.ctx
+@[simp] lemma AxiomT.ctx.includes_AxiomT : (AxiomT p) ∈ 𝐓 := by simp [ctx];
+
+@[simp] abbrev AxiomB := p ⟶ □◇p
+def AxiomB.ctx : Set F := { AxiomB p | p }
+notation "𝐁" => AxiomB.ctx
+@[simp] lemma AxiomB.ctx.includes_AxiomB : (AxiomB p) ∈ 𝐁 := by simp [ctx];
+
+@[simp] abbrev AxiomD := □p ⟶ ◇p
+def AxiomD.ctx : Set F := { AxiomD p | p }
+notation "𝐃" => AxiomD.ctx
+@[simp] lemma AxiomD.ctx.includes_AxiomD : (AxiomD p) ∈ 𝐃 := by simp [ctx];
+
+@[simp] abbrev Axiom4 := □p ⟶ □□p
+def Axiom4.ctx : Set F := { Axiom4 p | p }
+notation "𝟒" => Axiom4.ctx
+@[simp] lemma Axiom4.ctx.includes_Axiom4 : (Axiom4 p) ∈ 𝟒 := by simp [ctx];
+
+@[simp] abbrev Axiom5 := ◇p ⟶ □◇p
+def Axiom5.ctx : Set F := { Axiom5 p | p }
+notation "𝟓" => Axiom5.ctx
+@[simp] lemma Axiom5.ctx.includes_Axiom5 : (Axiom5 p) ∈ 𝟓 := by simp [ctx];
+
+@[simp] abbrev AxiomL := □(□p ⟶ p) ⟶ □p
+def AxiomL.ctx : Set F := { AxiomL p | p }
+notation "𝐋" => AxiomL.ctx
+@[simp] lemma AxiomL.ctx.includes_AxiomL : (AxiomL p) ∈ 𝐋 := by simp [ctx];
+
+@[simp] abbrev AxiomDot2 := ◇□p ⟶ □◇p
+def AxiomDot2.ctx : Set F := { AxiomDot2 p | p }
+notation ".𝟐" => AxiomDot2.ctx
+@[simp] lemma AxiomDot2.ctx.includes_AxiomDot2 : (AxiomDot2 p) ∈ .𝟐 := by simp [ctx];
+
+@[simp] abbrev AxiomDot3 := □(□p ⟶ □q) ⋎ □(□q ⟶ □p)
+def AxiomDot3.ctx : Set F := { AxiomDot3 p q | (p) (q) }
+notation ".𝟑" => AxiomDot3.ctx
+@[simp] lemma AxiomDot3.ctx.includes_AxiomDot3 : (AxiomDot3 p q) ∈ .𝟑 := by simp [ctx]; aesop;
+
+@[simp] abbrev AxiomGrz := □(□(p ⟶ □p) ⟶ p) ⟶ p
+def AxiomGrz.ctx : Set F := { AxiomGrz p | p }
+notation "𝐆𝐫𝐳" => AxiomGrz.ctx
+@[simp] lemma AxiomGrz.ctx.includes_AxiomGrz : (AxiomGrz p) ∈ 𝐆𝐫𝐳 := by simp [ctx];
+
+@[simp] abbrev AxiomM := (□◇p ⟶ ◇□p)
+def AxiomM.ctx : Set F := { AxiomM p | p }
+notation "𝐌" => AxiomM.ctx
+@[simp] lemma AxiomM.ctx.includes_AxiomM : (AxiomM p) ∈ 𝐌 := by simp [ctx];
+
+@[simp] abbrev AxiomCD := ◇p ⟶ □p
+def AxiomCD.ctx : Set F := { AxiomCD p | p }
+notation "𝐂𝐃" => AxiomCD.ctx
+@[simp] lemma AxiomCD.ctx.includes_AxiomCD : (AxiomCD p) ∈ 𝐂𝐃 := by simp [ctx];
+
+@[simp] abbrev AxiomC4 := □□p ⟶ □p
+def AxiomC4.ctx : Set F := { AxiomC4 p | p }
+notation "𝐂𝟒" => AxiomC4.ctx
+@[simp] lemma AxiomC4.ctx.includesAxiomC4 : (AxiomC4 p) ∈ 𝐂𝟒 := by simp [ctx];
+
+end Axioms
+
+
+section Logics
+
+abbrev LogicK.ctx : Set F := 𝐊
+
+abbrev LogicKD.ctx : Set F := 𝐊 ∪ 𝐃
+abbrev LogicKD4.ctx : Set F := 𝐊 ∪ 𝐃 ∪ 𝟒
+abbrev LogicKD5.ctx : Set F := 𝐊 ∪ 𝐃 ∪ 𝟓
+abbrev LogicKDB.ctx : Set F := 𝐊 ∪ 𝐃 ∪ 𝐁
+abbrev LogicKD45.ctx : Set F := 𝐊 ∪ 𝐃 ∪ 𝟒 ∪ 𝟓
+
+abbrev LogicKT.ctx : Set F := 𝐊 ∪ 𝐓
+abbrev LogicKTB.ctx : Set F := 𝐊 ∪ 𝐓 ∪ 𝐁
+abbrev LogicKT4.ctx : Set F := 𝐊 ∪ 𝐓 ∪ 𝟒
+abbrev LogicKT5.ctx : Set F := 𝐊 ∪ 𝐓 ∪ 𝟓
+
+abbrev LogicKB.ctx : Set F := 𝐊 ∪ 𝐁
+abbrev LogicKB5.ctx : Set F := 𝐊 ∪ 𝐁 ∪ 𝟓
+
+abbrev LogicK4.ctx : Set F := 𝐊 ∪ 𝟒
+abbrev LogicK45.ctx : Set F := 𝐊 ∪ 𝟒 ∪ 𝟓
+
+abbrev LogicK5.ctx : Set F := 𝐊 ∪ 𝟓
+
+/-- equals to `𝐊 ∪ 𝐓 ∪ 𝟒`  -/
+abbrev LogicS4.ctx : Set F := LogicKT4.ctx
+notation "𝐒𝟒" => LogicS4.ctx
+
+@[simp] lemma LogicS4.ctx.subsets_K : 𝐊 ⊆ (𝐒𝟒 : Set F) := by apply Set.subset_triunion₁
+@[simp] lemma LogicS4.ctx.subsets_T : 𝐓 ⊆ (𝐒𝟒 : Set F) := by apply Set.subset_triunion₂
+@[simp] lemma LogicS4.ctx.subsets_4 : 𝟒 ⊆ (𝐒𝟒 : Set F) := by apply Set.subset_triunion₃
+
+/-- equals to `𝐊 ∪ 𝐓 ∪ 𝟓` -/
+abbrev LogicS5.ctx : Set F := LogicKT5.ctx
+notation "𝐒𝟓" => LogicS5.ctx
+
+@[simp] lemma LogicS5.ctx.subsets_K : 𝐊 ⊆ (𝐒𝟓 : Set F) := by apply Set.subset_triunion₁
+@[simp] lemma LogicS5.ctx.subsets_T : 𝐓 ⊆ (𝐒𝟓 : Set F) := by apply Set.subset_triunion₂
+@[simp] lemma LogicS5.ctx.subsets_5 : 𝟓 ⊆ (𝐒𝟓 : Set F) := by apply Set.subset_triunion₃
+
+abbrev LogicGL.ctx : Set F := 𝐊 ∪ 𝐋
+notation "𝐆𝐋" => LogicGL.ctx
+
+@[simp] lemma LogicGL.ctx.subsets_K : 𝐊 ⊆ (𝐆𝐋 : Set F) := by aesop;
+@[simp] lemma LogicGL.ctx.subsets_L : 𝐋 ⊆ (𝐆𝐋 : Set F) := by aesop;
+
+abbrev LogicS4Dot2.ctx : Set F := 𝐒𝟒 ∪ .𝟐
+notation "𝐒𝟒.𝟐" => LogicS4Dot2.ctx
+
+@[simp] lemma LogicS4Dot2.ctx.subsets_S4 : 𝐒𝟒 ⊆ (𝐒𝟒.𝟐 : Set F) := by aesop;
+@[simp] lemma LogicS4Dot2.ctx.subsets_Dot2 : .𝟐 ⊆ (𝐒𝟒.𝟐 : Set F) := by aesop;
+
+abbrev LogicS4Dot3.ctx : Set F := 𝐒𝟒 ∪ .𝟑
+notation "𝐒𝟒.𝟑" => LogicS4Dot3.ctx
+
+@[simp] lemma LogicS4Dot3.ctx.subsets_S4 : 𝐒𝟒 ⊆ (𝐒𝟒.𝟑 : Set F) := by aesop;
+@[simp] lemma LogicS4Dot3.ctx.subsets_Dot3 : .𝟑 ⊆ (𝐒𝟒.𝟑 : Set F) := by aesop;
+
+abbrev LogicS4Grz.ctx : Set F := 𝐒𝟒 ∪ 𝐆𝐫𝐳
+notation "𝐒𝟒𝐆𝐫𝐳" => LogicS4Grz.ctx
+
+@[simp] lemma LogicS4Grz.ctx.subsets_S4 : 𝐒𝟒 ⊆ (𝐒𝟒𝐆𝐫𝐳 : Set F) := by aesop;
+@[simp] lemma LogicS4Grz.ctx.subsets_Grz : 𝐆𝐫𝐳 ⊆ (𝐒𝟒𝐆𝐫𝐳 : Set F) := by aesop;
+
+end Logics
+
+end LO.Modal
